Add guards

ShadowInterpMatchGuard.v
@@ -14,7 +14,7 @@ Inductive vec {A : Type} : nat -> Type :=
   | vcons {n} (hd : A) (tl : vec n) : vec (S n)
 .
 
-Section vec_IND.
+Section VEC_IND.
   Context {A : Type}.
   Context (P : forall n, @vec A n -> Prop).
   Context (Pnil : P 0 vnil)
@@ -25,13 +25,13 @@ Section vec_IND.
     | vnil => Pnil
     | @vcons _ n' hd tl => Pcons n' hd tl (vec_ind tl)
     end.
-End vec_IND.
+End VEC_IND.
 
 Declare Scope vec_scope.
 Delimit Scope vec_scope with vec.
 Infix "::" := vcons.
 Notation "[ ]" := vnil (format "[ ]") : vec_scope.
-Notation "[ x ]" := (vcons x nil) : vec_scope.
+Notation "[ x ]" := (vcons x vnil) : vec_scope.
 Notation "[ x ; y ; .. ; z ]" := (vcons x (vcons y .. (vcons z vnil) ..)) : vec_scope.
 
 Arguments vec : clear implicits.
@@ -72,16 +72,46 @@ Definition In_vec {A} (x : A) :=
     | hd :: tl => x = hd \/ In tl
     end%vec.
 
+Fixpoint map_vec_In {A B n} (l : vec A n) (f : forall x, In_vec x l -> B) {struct l} : vec B n.
+Proof.
+  destruct l.
+  - exact vnil.
+  - apply vcons.
+    + eapply (f hd _).
+    + eapply (map_vec_In _ _ _ l _).
+      Unshelve.
+      simpl. left; reflexivity.
+      intros. eapply f. simpl. eauto.
+Defined.
+
 Variant cstr_name : nat -> Type :=
   | Zero : cstr_name 0
   | Succ : cstr_name 1
+  | Cons : cstr_name 2
+  | One : cstr_name 0
 .
+
+Definition eqb_cstr {m n} (c1 : cstr_name m) (c2 : cstr_name n) :=
+  match c1, c2 with
+  | Zero, Zero | Succ, Succ | Cons, Cons | One, One => true
+  | Zero, _ | Succ, _ | Cons, _ | One, _ => false
+  end.
 
 Record cstr_type :=
   {
     cs_arity : nat;
     cs_name : cstr_name cs_arity;
   }.
+
+Lemma eqb_cstr_eq (c1 c2 : cstr_type) :
+  eqb_cstr c1.(cs_name) c2.(cs_name) = true <-> c1 = c2.
+Proof.
+  destruct c1, c2; simpl;
+  match goal with
+  | |- context [eqb_cstr ?x ?y] => destruct x, y
+  end; simpl;
+  split; intro EQ; inversion EQ; auto.
+Qed.
 
 Record cstr {V : Type} := mkCstr
   {
@@ -105,78 +135,78 @@ Record branch {B : Type} := mkBranch
 
 Inductive tm :=
   | Var (x : var)
-  | Fn (x : var) (e : tm)
+  | Fn (x : var) (e : tm) (* λ x . e *)
   | App (f a : tm)
   | Link (m e : tm) (* m ⋊ e *)
   | Mt (* ε *)
   | Bind (x : var) (v m : tm) (* let rec x = v ; m *)
   | Cstr (args : @cstr tm) (* C e1 e2 ... en *)
   | Case (e : tm) (b : list (@branch tm))
-    (* match e with | C1 \vec{x1} => e1 | ... | Cn \vec{xn} => en end *)
+  (* match e with | C1 \vec{x1} => e1 | ... | Cn \vec{xn} => en end *)
 .
 
-Inductive wvl {vl} :=
-  | wvl_v (v : vl) (* v *)
-  | wvl_recv (v : vl) (* μ.v *)
+Inductive shdw {wvl} :=
+  | Init
+  | Read (s : shdw) (x : var)
+  | Call (s : shdw) (w : wvl)
+  | Dstr (s : shdw) (d : dstr)
+.
+
+Arguments shdw : clear implicits.
+
+Inductive nv {wvl} :=
+  | nv_mt (* • *)
+  | nv_sh (s : shdw wvl) (* [s] *)
+  | nv_bd (x : var) (w : wvl) (σ : nv) (* bound value *)
+.
+
+Arguments nv : clear implicits.
+
+Inductive vl {wvl K} :=
+  | vl_exp (σ : nv wvl)
+  | vl_sh (s : shdw wvl) (* s *)
+  | vl_clos (x : var) (k : K) (σ : nv wvl)
+  | vl_cstr (c : @cstr wvl)
+.
+
+Arguments vl : clear implicits.
+
+Inductive wvl {K} :=
+  | wvl_v (v : vl wvl K) (* v *)
+  | wvl_recv (v : vl wvl K) (* μ.v *)
   | wvl_bloc (n : nat) (* bound location *)
   | wvl_floc (ℓ : loc) (* free location *)
 .
 
 Arguments wvl : clear implicits.
 
-Inductive shdw {vl} :=
-  | Init
-  | Read (s : shdw) (x : var)
-  | Call (s : shdw) (v : vl)
-  | Dstr (s : shdw) (d : dstr)
+(* finite approximations *)
+Inductive trace :=
+  | Bot
+  | Wal (w : wvl trace)
+  | Match (s : shdw (wvl trace)) (b : list (cstr_type * trace))
+  | Guard (σ : nv (wvl trace)) (t : trace)
 .
-
-Arguments shdw : clear implicits.
-
-Inductive nv {vl} :=
-  | nv_mt (* • *)
-  | nv_sh (s : shdw vl) (* [s] *)
-  | nv_bd (x : var) (w : wvl vl) (σ : nv) (* bound value *)
-.
-
-Arguments nv : clear implicits.
-
-Inductive vl {K} :=
-  | vl_sh (s : shdw vl)
-  | vl_exp (σ : nv vl)
-  | vl_clos (x : var) (k : K) (σ : nv vl)
-  | vl_cstr (c : @cstr (wvl vl))
-.
-
-Arguments vl : clear implicits.
 
 (*
 Variant traceF trace :=
   | Bot
-  | Wal (w : (wvl (vl (list trace))))
-  | Match (v : shdw (vl (list trace))) (c : cstr_type) (k : trace)
-  | Guard (σ : nv (vl (list trace))) (k : trace)
+  | Wal (w : wvl trace)
+  | Match (s : shdw (wvl trace)) (b : list (cstr_type * trace))
+  | Guard (σ : nv (wvl trace)) (t : trace)
 .
 
-CoInductive trace := mkTrace { _observe : traceF trace }.
+CoInductive trace := mkTrace { _obs_tr : traceF trace }.
 *)
 
-(* finite approximations *)
-Inductive trace :=
-  | Bot
-  | Wal (w : wvl (vl (list trace)))
-  | Match (s : shdw (vl (list trace))) (c : cstr_type) (k : trace)
-  | Guard (σ : nv (vl (list trace))) (k : trace)
-.
+Definition walue := wvl trace.
+Definition value := vl walue trace.
+Definition shadow := shdw walue.
+Definition env := nv walue.
 
-Definition value := vl (list trace).
-Definition walue := wvl value.
-Definition shadow := shdw value.
-Definition env := nv value.
-
-Section pre_val_IND.
+Section PRE_VAL_IND.
   Context {K : Type}.
-  Context (Pwvl : wvl (vl K) -> Prop) (Pnv : nv (vl K) -> Prop) (Pvl : vl K -> Prop) (Pshdw : shdw (vl K) -> Prop).
+  Context (Pwvl : wvl K -> Prop) (Pnv : nv (wvl K) -> Prop) (Pvl : vl (wvl K) K -> Prop) (Pshdw : shdw (wvl K) -> Prop).
   Context (Pwvl_v : forall v, Pvl v -> Pwvl (wvl_v v))
           (Pwvl_recv : forall v, Pvl v -> Pwvl (wvl_recv v))
           (Pwvl_bloc : forall n, Pwvl (wvl_bloc n))
@@ -184,50 +214,42 @@ Section pre_val_IND.
   Context (Pnv_mt : Pnv nv_mt)
           (Pnv_sh : forall s, Pshdw s -> Pnv (nv_sh s))
           (Pnv_bd : forall x w σ, Pwvl w -> Pnv σ -> Pnv (nv_bd x w σ)).
-  Context (Pvl_sh : forall s, Pshdw s -> Pvl (vl_sh s))
-          (Pvl_exp : forall σ, Pnv σ -> Pvl (vl_exp σ))
+  Context (Pvl_exp : forall σ, Pnv σ -> Pvl (vl_exp σ))
+          (Pvl_sh : forall s, Pshdw s -> Pvl (vl_sh s))
           (Pvl_clos : forall x k σ, Pnv σ -> Pvl (vl_clos x k σ))
           (Pvl_cstr : forall c (Pl : forall w, In_vec w c.(cs_args) -> Pwvl w),
             Pvl (vl_cstr c)).
   Context (PInit : Pshdw Init)
           (PRead : forall s x, Pshdw s -> Pshdw (Read s x))
-          (PCall : forall s v, Pshdw s -> Pvl v -> Pshdw (Call s v))
+          (PCall : forall s w, Pshdw s -> Pwvl w -> Pshdw (Call s w))
           (PDstr : forall s d, Pshdw s -> Pshdw (Dstr s d)).
 
-  Definition wvl_ind vl_ind w : Pwvl w :=
-    match w with
-    | wvl_v v => Pwvl_v v (vl_ind v)
-    | wvl_recv v => Pwvl_recv v (vl_ind v)
-    | wvl_bloc n => Pwvl_bloc n
-    | wvl_floc ℓ => Pwvl_floc ℓ
-    end.
-
-  Definition shdw_ind vl_ind :=
+  Definition shdw_ind wvl_ind :=
     fix shdw_ind s : Pshdw s :=
     match s with
     | Init => PInit
     | Read s x => PRead s x (shdw_ind s)
-    | Call s v => PCall s v (shdw_ind s) (vl_ind v)
+    | Call s w => PCall s w (shdw_ind s) (wvl_ind w)
     | Dstr s d => PDstr s d (shdw_ind s)
     end.
 
-  Definition nv_ind vl_ind :=
+  Definition nv_ind wvl_ind :=
     fix nv_ind σ : Pnv σ :=
     match σ with
     | nv_mt => Pnv_mt
-    | nv_sh s => Pnv_sh s (shdw_ind vl_ind s)
-    | nv_bd x w σ => Pnv_bd x w σ (wvl_ind vl_ind w) (nv_ind σ)
+    | nv_sh s => Pnv_sh s (shdw_ind wvl_ind s)
+    | nv_bd x w σ => Pnv_bd x w σ (wvl_ind w) (nv_ind σ)
     end.
 
-  Fixpoint vl_ind v : Pvl v.
+  Definition vl_ind (wvl_ind : forall w, Pwvl w) : forall v, Pvl v.
   Proof.
     refine (
-    let wvl_ind := wvl_ind vl_ind in
-    let shdw_ind := shdw_ind vl_ind in
-    let nv_ind := nv_ind vl_ind in
+    let shdw_ind := shdw_ind wvl_ind in
+    let nv_ind := nv_ind wvl_ind in
+    fix vl_ind v :=
     match v with
-    | vl_sh s => Pvl_sh s (shdw_ind s)
     | vl_exp σ => Pvl_exp σ (nv_ind σ)
+    | vl_sh s => Pvl_sh s (shdw_ind s)
     | vl_clos x k σ => Pvl_clos x k σ (nv_ind σ)
     | vl_cstr c =>
       let fix in_vec {n} (l : vec _ n) w (IN : In_vec w l) {struct l} : Pwvl w :=
@@ -242,7 +264,15 @@ Section pre_val_IND.
     - destruct IN' as [IN' | IN'].
       + rewrite IN'. apply wvl_ind.
       + eapply in_vec. exact IN'.
-  Qed.
+  Defined.
+
+  Fixpoint wvl_ind w : Pwvl w :=
+    match w with
+    | wvl_v v => Pwvl_v v (vl_ind wvl_ind v)
+    | wvl_recv v => Pwvl_recv v (vl_ind wvl_ind v)
+    | wvl_bloc n => Pwvl_bloc n
+    | wvl_floc ℓ => Pwvl_floc ℓ
+    end.
 
   Lemma pre_val_ind :
     (forall w, Pwvl w) /\
@@ -250,14 +280,15 @@ Section pre_val_IND.
     (forall v, Pvl v) /\
     (forall s, Pshdw s).
   Proof.
-    eauto using (wvl_ind vl_ind), (nv_ind vl_ind), vl_ind, (shdw_ind vl_ind).
+    eauto using wvl_ind, (nv_ind wvl_ind), (vl_ind wvl_ind), (shdw_ind wvl_ind).
   Qed.
-End pre_val_IND.
+End PRE_VAL_IND.
 
 Local Notation "'⟨' 'μ' v '⟩'" := (wvl_recv v) (at level 60, right associativity, only printing).
+Local Notation "'⟨' n '⟩'" := (wvl_bloc n) (at level 60, right associativity, only printing).
 Local Notation "'⟨' v '⟩'" := (wvl_v v) (at level 60, right associativity, only printing).
-Local Notation "'⟨' 'λ' x k σ '⟩'" := (vl_clos x k σ) (at level 60, right associativity, only printing).
 Local Notation "'⟨' s '⟩'" := (vl_sh s) (at level 60, right associativity, only printing).
+Local Notation "'⟨' 'λ' x k σ '⟩'" := (vl_clos x k σ) (at level 60, right associativity, only printing).
 Local Notation "•" := (nv_mt) (at level 60, right associativity, only printing).
 Local Notation "'⟪' s '⟫'" := (nv_sh s) (at level 60, right associativity, only printing).
 Local Notation "'⟪' x ',' w '⟫' ';;' σ " := (nv_bd x w σ) (at level 60, right associativity, only printing).
@@ -272,20 +303,12 @@ Definition lift {A B : Type} (f : A -> option B) (x : option A) :=
 
 (** Operations for substitution *)
 (* open the bound location i with ℓ *)
-Definition open_loc_wvl f (i : nat) (ℓ : loc) (w : walue) : walue :=
-  match w with
-  | wvl_v v => wvl_v (f i ℓ v)
-  | wvl_recv v => wvl_recv (f (S i) ℓ v)
-  | wvl_bloc n => if Nat.eqb i n then wvl_floc ℓ else wvl_bloc n
-  | wvl_floc ℓ => wvl_floc ℓ
-  end.
-
 Definition open_loc_shdw f (i : nat) (ℓ : loc) :=
   fix open (s : shadow) : shadow :=
   match s with
   | Init => Init
   | Read s x => Read (open s) x
-  | Call s v => Call (open s) (f i ℓ v)
+  | Call s w => Call (open s) (f i ℓ w)
   | Dstr s d => Dstr (open s) d
   end.
 
@@ -295,41 +318,44 @@ Definition open_loc_nv f (i : nat) (ℓ : loc) :=
   | nv_mt => nv_mt
   | nv_sh s => nv_sh (open_loc_shdw f i ℓ s)
   | nv_bd x w σ' =>
-    nv_bd x (open_loc_wvl f i ℓ w) (open σ')
+    nv_bd x (f i ℓ w) (open σ')
   end.
 
-Fixpoint open_loc_value (i : nat) (ℓ : loc) (v : value) {struct v} :=
+Definition open_loc_vl f (i : nat) (ℓ : loc) :=
+  fix open (v : value) :=
   match v with
-  | vl_sh s => vl_sh (open_loc_shdw open_loc_value i ℓ s)
-  | vl_exp σ => vl_exp (open_loc_nv open_loc_value i ℓ σ)
-  | vl_clos x k σ => vl_clos x k (open_loc_nv open_loc_value i ℓ σ)
+  | vl_exp σ => vl_exp (open_loc_nv f i ℓ σ)
+  | vl_sh s => vl_sh (open_loc_shdw f i ℓ s)
+  | vl_clos x k σ => vl_clos x k (open_loc_nv f i ℓ σ)
   | vl_cstr c =>
     vl_cstr
     {|
       cs_type := c.(cs_type);
-      cs_args := map_vec (open_loc_wvl open_loc_value i ℓ) c.(cs_args)
+      cs_args := map_vec (f i ℓ) c.(cs_args)
     |}
   end.
 
-Definition open_loc_walue := open_loc_wvl open_loc_value.
-Definition open_loc_env := open_loc_nv open_loc_value.
-Definition open_loc_shadow := open_loc_shdw open_loc_value.
-
-(* close the free location ℓ with the binding depth i *)
-Definition close_wvl f (i : nat) (ℓ : loc) (w : walue) : walue :=
+Fixpoint open_loc_walue (i : nat) (ℓ : loc) (w : walue) : walue :=
+  let open_loc_vl := open_loc_vl open_loc_walue in
+  let open_loc_shdw := open_loc_shdw open_loc_walue in
   match w with
-  | wvl_v v => wvl_v (f i ℓ v)
-  | wvl_recv v => wvl_recv (f (S i) ℓ v)
-  | wvl_bloc n => wvl_bloc n
-  | wvl_floc ℓ' => if Pos.eqb ℓ ℓ' then wvl_bloc i else wvl_floc ℓ'
+  | wvl_v v => wvl_v (open_loc_vl i ℓ v)
+  | wvl_recv v => wvl_recv (open_loc_vl (S i) ℓ v)
+  | wvl_bloc n => if Nat.eqb i n then wvl_floc ℓ else wvl_bloc n
+  | wvl_floc ℓ => wvl_floc ℓ
   end.
 
+Definition open_loc_value := open_loc_vl open_loc_walue.
+Definition open_loc_env := open_loc_nv open_loc_walue.
+Definition open_loc_shadow := open_loc_shdw open_loc_walue.
+
+(* close the free location ℓ with the binding depth i *)
 Definition close_shdw f (i : nat) (ℓ : loc) :=
   fix close (s : shadow) : shadow :=
   match s with
   | Init => Init
   | Read s x => Read (close s) x
-  | Call s v => Call (close s) (f i ℓ v)
+  | Call s w => Call (close s) (f i ℓ w)
   | Dstr s d => Dstr (close s) d
   end.
 
@@ -339,41 +365,44 @@ Definition close_nv f (i : nat) (ℓ : loc) :=
   | nv_mt => nv_mt
   | nv_sh s => nv_sh (close_shdw f i ℓ s)
   | nv_bd x w σ' =>
-    nv_bd x (close_wvl f i ℓ w) (close σ')
+    nv_bd x (f i ℓ w) (close σ')
   end.
 
-Fixpoint close_value (i : nat) (ℓ : loc) (v : value) : value :=
+Definition close_vl f (i : nat) (ℓ : loc) :=
+  fix close (v : value) : value :=
   match v with
-  | vl_sh s => vl_sh (close_shdw close_value i ℓ s)
-  | vl_exp σ => vl_exp (close_nv close_value i ℓ σ)
-  | vl_clos x k σ => vl_clos x k (close_nv close_value i ℓ σ)
+  | vl_exp σ => vl_exp (close_nv f i ℓ σ)
+  | vl_sh s => vl_sh (close_shdw f i ℓ s)
+  | vl_clos x k σ => vl_clos x k (close_nv f i ℓ σ)
   | vl_cstr c =>
     vl_cstr
     {|
       cs_type := c.(cs_type);
-      cs_args := map_vec (close_wvl close_value i ℓ) c.(cs_args);
+      cs_args := map_vec (f i ℓ) c.(cs_args);
     |}
   end.
 
-Definition close_walue := close_wvl close_value.
-Definition close_env := close_nv close_value.
-Definition close_shadow := close_shdw close_value.
-
-(* open the bound location i with u *)
-Definition open_wvl_wvl f (i : nat) (u : walue) (w : walue) : walue :=
+Fixpoint close_walue (i : nat) (ℓ : loc) (w : walue) : walue :=
+  let close_vl := close_vl close_walue in
+  let close_shdw := close_shdw close_walue in
   match w with
-  | wvl_v v => wvl_v (f i u v)
-  | wvl_recv v => wvl_recv (f (S i) u v)
-  | wvl_bloc n => if Nat.eqb i n then u else wvl_bloc n
-  | wvl_floc ℓ => wvl_floc ℓ
+  | wvl_v v => wvl_v (close_vl i ℓ v)
+  | wvl_recv v => wvl_recv (close_vl (S i) ℓ v)
+  | wvl_bloc n => wvl_bloc n
+  | wvl_floc ℓ' => if Pos.eqb ℓ ℓ' then wvl_bloc i else wvl_floc ℓ'
   end.
 
+Definition close_value := close_vl close_walue.
+Definition close_env := close_nv close_walue.
+Definition close_shadow := close_shdw close_walue.
+
+(* open the bound location i with u *)
 Definition open_wvl_shdw f (i : nat) (u : walue) :=
   fix open (s : shadow) : shadow :=
   match s with
   | Init => Init
   | Read s x => Read (open s) x
-  | Call s v => Call (open s) (f i u v)
+  | Call s w => Call (open s) (f i u w)
   | Dstr s d => Dstr (open s) d
   end.
 
@@ -383,40 +412,44 @@ Definition open_wvl_nv f (i : nat) (u : walue) :=
   | nv_mt => nv_mt
   | nv_sh s => nv_sh (open_wvl_shdw f i u s)
   | nv_bd x w σ' =>
-    nv_bd x (open_wvl_wvl f i u w) (open σ')
+    nv_bd x (f i u w) (open σ')
   end.
 
-Fixpoint open_wvl_value (i : nat) (u : walue) (v : value) {struct v} :=
+Definition open_wvl_vl f (i : nat) (u : walue) :=
+  fix open (v : value) :=
   match v with
-  | vl_sh s => vl_sh (open_wvl_shdw open_wvl_value i u s)
-  | vl_exp σ => vl_exp (open_wvl_nv open_wvl_value i u σ)
-  | vl_clos x k σ => vl_clos x k (open_wvl_nv open_wvl_value i u σ)
+  | vl_exp σ => vl_exp (open_wvl_nv f i u σ)
+  | vl_sh s => vl_sh (open_wvl_shdw f i u s)
+  | vl_clos x k σ => vl_clos x k (open_wvl_nv f i u σ)
   | vl_cstr c =>
     vl_cstr
     {|
       cs_type := c.(cs_type);
-      cs_args := map_vec (open_wvl_wvl open_wvl_value i u) c.(cs_args)
+      cs_args := map_vec (f i u) c.(cs_args)
     |}
   end.
 
-Definition open_wvl_walue := open_wvl_wvl open_wvl_value.
-Definition open_wvl_env := open_wvl_nv open_wvl_value.
-Definition open_wvl_shadow := open_wvl_shdw open_wvl_value.
+Fixpoint open_wvl_walue (i : nat) (u : walue) (w : walue) : walue :=
+  let open_wvl_vl := open_wvl_vl open_wvl_walue in
+  let open_wvl_shdw := open_wvl_shdw open_wvl_walue in
+  match w with
+  | wvl_v v => wvl_v (open_wvl_vl i u v)
+  | wvl_recv v => wvl_recv (open_wvl_vl (S i) u v)
+  | wvl_bloc n => if Nat.eqb i n then u else wvl_bloc n
+  | wvl_floc ℓ => wvl_floc ℓ
+  end.
+
+Definition open_wvl_value := open_wvl_vl open_wvl_walue.
+Definition open_wvl_env := open_wvl_nv open_wvl_walue.
+Definition open_wvl_shadow := open_wvl_shdw open_wvl_walue.
 
 (* allocate fresh locations *)
-Definition alloc_wvl f (w : walue) : positive :=
-  match w with
-  | wvl_v v | wvl_recv v => f v
-  | wvl_bloc _ => 1
-  | wvl_floc ℓ => Pos.succ ℓ
-  end%positive.
-
 Definition alloc_shdw f :=
   fix alloc (s : shadow) : positive :=
   match s with
   | Init => xH
   | Read s x => alloc s
-  | Call s v => Pos.max (alloc s) (f v)
+  | Call s w => Pos.max (alloc s) (f w)
   | Dstr s d => alloc s
   end.
 
@@ -425,35 +458,39 @@ Definition alloc_nv f :=
   match σ with
   | nv_mt => xH
   | nv_sh s => alloc_shdw f s
-  | nv_bd _ w σ' => Pos.max (alloc_wvl f w) (alloc σ')
+  | nv_bd _ w σ' => Pos.max (f w) (alloc σ')
   end.
 
-Fixpoint alloc_value (v : value) : positive :=
+Definition alloc_vl f :=
+  fix alloc (v : value) : positive :=
   match v with
-  | vl_sh s => alloc_shdw alloc_value s
-  | vl_exp σ | vl_clos _ _ σ => alloc_nv alloc_value σ
+  | vl_exp σ | vl_clos _ _ σ => alloc_nv f σ
+  | vl_sh s => alloc_shdw f s
   | vl_cstr c =>
-    let for_each acc w := Pos.max acc (alloc_wvl alloc_value w) in
+    let for_each acc w := Pos.max acc (f w) in
     fold_vec for_each c.(cs_args) xH
   end.
 
-Definition alloc_walue := alloc_wvl alloc_value.
-Definition alloc_env := alloc_nv alloc_value.
-Definition alloc_shadow := alloc_shdw alloc_value.
+Fixpoint alloc_walue (w : walue) : positive :=
+  let alloc_vl := alloc_vl alloc_walue in
+  let alloc_shdw := alloc_shdw alloc_walue in
+  match w with
+  | wvl_v v | wvl_recv v => alloc_vl v
+  | wvl_bloc _ => 1
+  | wvl_floc ℓ => Pos.succ ℓ
+  end%positive.
+
+Definition alloc_value := alloc_vl alloc_walue.
+Definition alloc_env := alloc_nv alloc_walue.
+Definition alloc_shadow := alloc_shdw alloc_walue.
 
 (* term size *)
-Definition size_wvl f (w : walue) :=
-  match w with
-  | wvl_v v | wvl_recv v => S (f v)
-  | wvl_bloc _ | wvl_floc _ => O
-  end.
-
 Definition size_shdw f :=
   fix size (s : shadow) :=
   match s with
   | Init => O
   | Read s x => S (size s)
-  | Call s v => S (Nat.max (size s) (f v))
+  | Call s w => S (Nat.max (size s) (f w))
   | Dstr s d => S (size s)
   end.
 
@@ -462,21 +499,30 @@ Definition size_nv f :=
   match σ with
   | nv_mt => O
   | nv_sh s => S (size_shdw f s)
-  | nv_bd _ w σ' => S (Nat.max (size_wvl f w) (size σ'))
+  | nv_bd _ w σ' => S (Nat.max (f w) (size σ'))
   end.
 
-Fixpoint size_value (v : value) :=
+Definition size_vl f :=
+  fix size (v : value) :=
   match v with
-  | vl_sh s => S (size_shdw size_value s)
-  | vl_exp σ | vl_clos _ _ σ => S (size_nv size_value σ)
+  | vl_exp σ | vl_clos _ _ σ => S (size_nv f σ)
+  | vl_sh s => S (size_shdw f s)
   | vl_cstr c =>
-    let for_each acc w := Nat.max acc (size_wvl size_value w) in
+    let for_each acc w := Nat.max acc (f w) in
     S (fold_vec for_each c.(cs_args) O)
   end.
 
-Definition size_walue := size_wvl size_value.
-Definition size_env := size_nv size_value.
-Definition size_shadow := size_shdw size_value.
+Fixpoint size_walue (w : walue) :=
+  let size_vl := size_vl size_walue in
+  let size_shdw := size_shdw size_walue in
+  match w with
+  | wvl_v v | wvl_recv v => S (size_vl v)
+  | wvl_bloc _ | wvl_floc _ => O
+  end.
+
+Definition size_value := size_vl size_walue.
+Definition size_env := size_nv size_walue.
+Definition size_shadow := size_shdw size_walue.
 
 Definition open_loc_size_eq_wvl w :=
   forall n ℓ, size_walue w = size_walue (open_loc_walue n ℓ w).
@@ -490,8 +536,8 @@ Definition open_loc_size_eq_shdw s :=
 Lemma open_loc_size_eq_vec m n ℓ (l : vec _ m) :
   forall acc
     (IH : forall w, In_vec w l -> open_loc_size_eq_wvl w),
-    fold_vec (fun acc w => Nat.max acc (size_wvl size_value w)) l acc =
-    fold_vec (fun acc w => Nat.max acc (size_wvl size_value w))
+    fold_vec (fun acc w => Nat.max acc (size_walue w)) l acc =
+    fold_vec (fun acc w => Nat.max acc (size_walue w))
       (map_vec (open_loc_walue n ℓ) l) acc.
 Proof.
   induction l; intros; simpl; auto.
@@ -527,74 +573,272 @@ Definition unroll (w : walue) : option value :=
   | wvl_bloc _ | wvl_floc _ => None
   end.
 
-Definition eval (link : nv -> vl -> option vl) :=
-  fix eval (e : tm) : list trace :=
-  match e with
-  | Var x => Some (vl_sh (Read Init x))
-  | Fn x M => Some (vl_clos x (eval M) (nv_sh Init))
-  | App M N =>
-    let foldM fn :=
-      let foldN arg :=
-        match fn with
-        | vl_clos x B σ =>
-          lift (link (nv_bval x (wvl_v arg) σ)) B
-        | vl_sh (SuccS _) | vl_sh (PredS _) => None
-        | vl_sh fn => Some (vl_sh (Call fn arg))
-        | vl_exp _ | vl_nat _ => None
+Local Definition dstr_helper1 m n k :
+  n <= m -> S k <= m -> k <= m.
+Proof. lia. Qed.
+
+Local Definition dstr_helper2 m n k :
+  n <= m -> S k <= m -> S (m - S k) <= m.
+Proof. lia. Qed.
+
+Definition dstr_shadow {B} (s : shadow) (b : @branch B) : env.
+Proof.
+  refine (
+  let arity := b.(br_cstr).(cs_arity) in
+  let fix for_each {n} (l : vec var n) (LE : n <= arity) acc {struct l} :=
+    match l as l' in vec _ m return m <= arity -> _ with
+    | [] => fun _ => acc
+    | hd :: tl => _
+    end%vec LE
+  in for_each b.(br_vars) _ (nv_sh Init)); constructor.
+  Unshelve. intro LE'.
+  eapply for_each; [exact tl | eapply dstr_helper1; eauto | eapply nv_bd].
+  - exact hd.
+  - apply wvl_v. apply vl_sh.
+    match goal with
+    | _ : context [S ?m] |- _ =>
+    refine (Dstr s
+      {|
+        ds_type := b.(br_cstr);
+        ds_idx := b.(br_cstr).(cs_arity) - (S m);
+        ds_valid := _
+      |})
+    end; eapply dstr_helper2; eauto.
+  - exact acc.
+Defined.
+
+Definition dstr_cstr {B} (c : @cstr walue) (b : @branch B) : option env.
+Proof.
+  refine(
+  let b_name := b.(br_cstr).(cs_name) in
+  let c_name := c.(cs_type).(cs_name) in
+  match eqb_cstr c_name b_name as b return eqb_cstr c_name b_name = b -> _ with
+  | true => fun EQ =>
+    let fix add_binding {m n} acc (xs : vec _ m) (ws : vec _ n) (EQ : m = n) :=
+      match xs in vec _ m' return m' = n -> _ with
+      | [] => fun _ => acc
+      | x :: xs => fun EQ =>
+        match ws in vec _ n' return m = n' -> _ with
+        | [] => fun CONTRA => _
+        | w :: ws => fun RR =>
+          add_binding (nv_bd x w acc) xs ws _
+        end _
+      end EQ
+    in Some (add_binding (nv_sh Init) b.(br_vars) c.(cs_args) _)
+  | false => fun _ => None
+  end%vec eq_refl).
+  - subst b_name. subst c_name.
+    rewrite eqb_cstr_eq in *.
+    rewrite EQ. reflexivity.
+    Unshelve.
+    all:congruence.
+Defined.
+
+Definition map_branches (k : trace -> trace) b :=
+  let for_branch (b : cstr_type * trace) :=
+    let (c, t) := b in (c, k t)
+  in List.map for_branch b
+.
+
+Definition bind (k : walue -> trace) : trace -> trace :=
+  fix bind t :=
+    match t with
+    | Bot => Bot
+    | Wal w => k w
+    | Match s b => Match s (map_branches bind b)
+    | Guard σ t => Guard σ (bind t)
+    end.
+
+Definition dstr_trace (d : dstr) : trace -> trace.
+Proof.
+  refine (
+  let k w :=
+    match unroll w with
+    | Some (vl_sh s) => Wal (wvl_v (vl_sh (Dstr s d)))
+    | Some (vl_cstr c) =>
+      let c_name := c.(cs_type).(cs_name) in
+      let d_name := d.(ds_type).(cs_name) in
+      match eqb_cstr c_name d_name as b return eqb_cstr c_name d_name = b -> _ with
+      | true => fun EQ => Wal (get_idx c.(cs_args) d.(ds_idx) _)
+      | false => fun _ => Bot
+      end eq_refl
+    | _ => Bot
+    end
+  in bind k);
+  subst c_name; subst d_name;
+  rewrite eqb_cstr_eq in *;
+  rewrite EQ; exact d.(ds_valid).
+Defined.
+
+Definition test_dstr_shadow := dstr_shadow Init
+  {|
+    br_cstr := {| cs_name := Cons; cs_arity := 2 |};
+    br_vars := ["x"; "y"]%vec;
+    br_body := tt;
+  |}.
+
+Definition test_dstr_cstr := dstr_cstr
+  {|
+    cs_type := {| cs_name := Cons; cs_arity := 2 |};
+    cs_args := [wvl_bloc 0; wvl_bloc 1]%vec;
+  |}
+  {|
+    br_cstr := {| cs_name := Cons; cs_arity := 2 |};
+    br_vars := ["x"; "y"]%vec;
+    br_body := tt;
+  |}.
+
+(*
+Eval vm_compute in test_dstr_shadow.
+Eval vm_compute in test_dstr_cstr.
+ *)
+
+Compute dstr_trace
+  {|
+    ds_type := {| cs_name := Cons; cs_arity := 2 |};
+    ds_idx := 1;
+    ds_valid := ltac:(repeat constructor);
+  |}
+  (Wal (wvl_v (vl_cstr
+  {|
+    cs_type := {| cs_name := Cons; cs_arity := 2 |};
+    cs_args := [wvl_bloc 0; wvl_bloc 1]%vec;
+  |}))).
+
+(* type of fold_left *)
+(* forall A B, (A -> B -> A) -> list B -> A -> A *)
+
+Definition cstr_trace (c : @cstr trace) : trace :=
+  let arity := c.(cs_type).(cs_arity) in
+  let fix fold_arg {n} (v : vec trace n) (k : vec walue n -> vec walue arity) {struct v} :=
+    match v in vec _ m return (vec walue m -> vec walue arity) -> _ with
+    | [] => fun k =>
+      Wal (wvl_v (vl_cstr {| cs_type := c.(cs_type) ; cs_args := k vnil |}))
+    | hd :: tl => fun k =>
+      let check_trace w := fold_arg tl (fun v => k (w :: v))
+      in bind check_trace hd
+    end%vec k
+  in fold_arg c.(cs_args) (fun v => v).
+
+Definition link_trace (link : walue -> trace) (k : walue -> trace) : trace -> trace :=
+  fix link_trace t :=
+    match t with
+    | Bot => Bot
+    | Wal w => bind k (link w)
+    | Match s b =>
+      let check_match w :=
+        match unroll w with
+        | Some (vl_sh s) => Match s (map_branches link_trace b)
+        | Some (vl_cstr c) =>
+          let fold_branch acc (b : cstr_type * trace) :=
+            let (c', t) := b in
+            match acc with
+            | None =>
+              if eqb_cstr c.(cs_type).(cs_name) c'.(cs_name)
+              then Some (link_trace t) else None
+            | Some t => Some t
+            end
+          in match List.fold_left fold_branch b None with
+          | None => Bot
+          | Some t => t
+          end
+        | _ => Bot
         end
-      in lift foldN (eval N)
-    in lift foldM (eval M)
-  | Link M N =>
-    let foldM m :=
-      let foldN cli :=
-        match m with
-        | vl_exp σ => link σ cli
-        | vl_sh (SuccS _) | vl_sh (PredS _) => None
-        | vl_sh m => link (nv_sh m) cli
-        | vl_clos _ _ _ | vl_nat _ => None
+      in bind check_match (link (wvl_v (vl_sh s)))
+    | Guard σ t =>
+      let check_guard w :=
+        match unroll w with
+        | Some (vl_sh s) => Guard (nv_sh s) (link_trace t)
+        | Some (vl_exp σ) => Guard σ (link_trace t)
+        | _ => Bot
         end
-      in lift foldN (eval N)
-    in lift foldM (eval M)
-  | Mt => Some (vl_exp nv_mt)
-  | Bind x M N =>
-    let foldM v :=
-      let w := wvl_recv (close_value 0 xH v) in
-      let foldN m :=
-        match m with
-        | vl_exp σ => Some (vl_exp (nv_bval x w σ))
-        | vl_sh (SuccS _) | vl_sh (PredS _) => None
-        | vl_sh s => Some (vl_exp (nv_bval x w (nv_sh s)))
-        | vl_clos _ _ _ | vl_nat _ => None
-        end
-      in lift foldN
-        (lift (link (nv_bval x w (nv_sh Init))) (eval N))
-    in lift foldM
-      (lift (link (nv_floc x xH (nv_sh Init))) (eval M))
-  | Zero => Some (vl_nat 0)
-  | Succ N =>
-    let foldN n :=
-      match n with
-      | vl_nat n => Some (vl_nat (S n))
-      | vl_sh s => Some (vl_sh (SuccS s))
-      | vl_exp _ | vl_clos _ _ _ => None
+      in bind check_guard (link (wvl_v (vl_exp σ)))
+    end.
+
+Definition read_trace x :=
+  let read w :=
+    match unroll w with
+    | Some (vl_sh s) => Wal (wvl_v (vl_sh (Read s x)))
+    | Some (vl_exp σ) =>
+      match read_env σ x with
+      | Some w => Wal w
+      | None => Bot
       end
-    in lift foldN (eval N)
-  | Case E M x N =>
-    let foldE e :=
-      match e with
-      | vl_nat O => eval M
-      | vl_nat (S n) =>
-        lift (link (nv_bval x (wvl_v (vl_nat n)) (nv_sh Init))) (eval N)
-      | vl_sh (SuccS s) =>
-        lift (link (nv_bval x (wvl_v (vl_sh s)) (nv_sh Init))) (eval N)
-      | vl_sh s =>
-        let vO := eval M in
-        let vS := lift (link (nv_bval x (wvl_v (vl_sh (PredS s))) (nv_sh Init))) (eval N) in
-        Some (vl_sh (CaseS s vO vS))
-      | vl_exp _ | vl_clos _ _ _ => None
+    | _ => Bot
+    end
+  in bind read.
+
+Definition call_trace
+  (link : env -> walue -> trace)
+  (fn arg : trace) : trace :=
+  let check_fn fn :=
+    match unroll fn with
+    | Some (vl_sh s) =>
+      let check_arg arg := Wal (wvl_v (vl_sh (Call s arg)))
+      in bind check_arg arg
+    | Some (vl_clos x t σ) =>
+      let check_arg arg :=
+        let σ' := nv_bd x arg σ
+        in link_trace (link σ') Wal t
+      in bind check_arg arg
+    | _ => Bot
+    end
+  in bind check_fn fn.
+
+Definition close_rec ℓ :=
+  let close w :=
+    match unroll w with
+    | Some v => Wal (wvl_recv (close_value 0 ℓ v))
+    | None => Bot
+    end
+  in bind close.
+
+Definition bd_trace x (w : trace) (σ : trace) :=
+  let check_bd w :=
+    let check_mod σ :=
+      match unroll σ with
+      | Some (vl_sh s) => Wal (wvl_v (vl_exp (nv_bd x w (nv_sh s))))
+      | Some (vl_exp σ) => Wal (wvl_v (vl_exp (nv_bd x w σ)))
+      | _ => Bot
       end
-    in lift foldE (eval E)
-  end.
+    in bind check_mod σ in
+  bind check_bd w.
+
+Definition clos_trace x k :=
+  let clos w :=
+    match unroll w with
+    | Some (vl_sh s) => Wal (wvl_v (vl_clos x k (nv_sh s)))
+    | Some (vl_exp σ) => Wal (wvl_v (vl_clos x k σ))
+    | _ => Bot
+    end
+  in bind clos.
+
+Definition filter_env :=
+  let filter w :=
+    match unroll w with
+    | Some (vl_sh s) => Wal (wvl_v (vl_exp (nv_sh s)))
+    | Some (vl_exp σ) => Wal (wvl_v (vl_exp σ))
+    | _ => Bot
+    end
+  in bind filter.
+
+Lemma fold_fact {n} (v : vec walue n) :
+  let fold acc w' := Nat.max acc (size_walue w') in
+  forall x y, x <= y -> x < S (fold_vec fold v y).
+Proof.
+  induction v; intros; simpl in *; [lia | apply IHv; subst fold; simpl; lia].
+Qed.
+
+Lemma link_helper {n} (v : vec walue n) :
+  let fold acc w' := Nat.max acc (size_walue w') in
+  forall m w (IN : In_vec w v),
+    size_walue w < S (fold_vec fold v m).
+Proof.
+  intro.
+  induction v; intros; simpl in *; [contradiction | destruct IN as [IN | IN]].
+  - subst. apply fold_fact. subst fold; simpl. lia.
+  - auto.
+Qed.
 
 Ltac t :=
   repeat match goal with
@@ -602,209 +846,240 @@ Ltac t :=
   | _ => progress simpl
   | RR : ?x = _ |- context [?x] => rewrite RR
   | |- context [size_value (open_loc_value ?n ?ℓ ?v)] =>
-    replace (size_value (open_loc_value n ℓ v)) with (size_vl v);
+    replace (size_value (open_loc_value n ℓ v)) with (size_value v);
     [|eapply open_loc_size_eq]
+  | _ => apply link_helper
   end.
 
 (* linking, up to n steps *)
-Fixpoint link (n : nat) (σ : nv) : vl -> option vl.
+Fixpoint link (n : nat) (σ : env) : walue -> trace.
 Proof.
   refine (
-  match n with 0 => (fun _ => None) | S n =>
+  match n with 0 => (fun _ => Bot) | S n =>
   let go :=
-  fix link_wvl w (ACC : Acc lt (size_wvl w)) {struct ACC} : option wvl :=
+  fix link_wvl w (ACC : Acc lt (size_walue w)) {struct ACC} : trace :=
     match w as w' return w = w' -> _ with
-    | wvl_v v => fun _ => lift (Some <*> wvl_v) (link_vl v (Acc_inv ACC _))
-    | wvl_recv v =>
-      fun _ =>
-      let ℓ := alloc_value v in
-      let recv v := Some (wvl_recv (close_value 0 ℓ v)) in
-      lift recv (link_vl (open_loc_value 0 ℓ v) (Acc_inv ACC _))
+    | wvl_v v => fun _ => link_vl v (Acc_inv ACC _)
+    | wvl_recv v => fun _ =>
+      let ℓ := Pos.max (alloc_value v) (alloc_env σ) in
+      close_rec ℓ (link_vl (open_loc_value 0 ℓ v) (Acc_inv ACC _))
+    | wvl_bloc n => fun _ => (* unreachable *) Bot
+    | wvl_floc ℓ => fun _ => Wal (wvl_floc ℓ)
     end eq_refl
-  with link_vl v (ACC : Acc lt (size_value v)) {struct ACC} : option vl :=
+  with link_vl v (ACC : Acc lt (size_value v)) {struct ACC} : trace :=
     match v as v' return v = v' -> _ with
-    | vl_clos x k σ' => fun _ => lift (Some <*> vl_clos x k) (link_nv σ' (Acc_inv ACC _))
-    | vl_exp σ' => fun _ => lift (Some <*> vl_exp) (link_nv σ' (Acc_inv ACC _))
+    | vl_clos x k σ' => fun _ =>
+      clos_trace x k (link_nv σ' (Acc_inv ACC _))
+    | vl_exp σ' => fun _ => link_nv σ' (Acc_inv ACC _)
     | vl_sh s => fun _ => link_shdw s (Acc_inv ACC _)
-    | vl_nat n => fun _ => Some (vl_nat n)
+    | vl_cstr c => fun _ =>
+      cstr_trace
+      {|
+        cs_type := c.(cs_type);
+        cs_args :=
+          map_vec_In c.(cs_args)
+            (fun w IN => link_wvl w (Acc_inv ACC _));
+      |}
     end eq_refl
-  with link_nv σ' (ACC : Acc lt (size_nv σ')) {struct ACC} : option nv :=
+  with link_nv σ' (ACC : Acc lt (size_env σ')) {struct ACC} : trace :=
     match σ' as σ'' return σ' = σ'' -> _ with
-    | nv_mt => fun _ => Some (nv_mt)
-    | nv_sh s =>
-      fun _ =>
-      let folds v :=
-        match v with
-        | vl_exp σ' => Some σ'
-        | vl_sh (SuccS _) | vl_sh (PredS _) => None
-        | vl_sh s' => Some (nv_sh s')
-        | vl_clos _ _ _ | vl_nat _ => None
-        end
-      in lift folds (link_shdw s (Acc_inv ACC _))
-    | nv_bloc _ _ _ => (* unreachable *) fun _ => None
-    | nv_floc x ℓ σ' => fun _ => lift (Some <*> nv_floc x ℓ) (link_nv σ' (Acc_inv ACC _))
-    | nv_bval x w σ' =>
-      fun _ =>
-      let foldw w := lift (Some <*> nv_bval x w) (link_nv σ' (Acc_inv ACC _))
-      in lift foldw (link_wvl w (Acc_inv ACC _))
+    | nv_mt => fun _ => Wal (wvl_v (vl_exp nv_mt))
+    | nv_sh s => fun _ =>
+      filter_env (link_shdw s (Acc_inv ACC _))
+    | nv_bd x w σ' => fun _ =>
+      bd_trace x
+        (link_wvl w (Acc_inv ACC _))
+        (link_nv σ' (Acc_inv ACC _))
     end eq_refl
-  with link_shdw s (ACC : Acc lt (size_shdw s)) {struct ACC} : option vl :=
+  with link_shdw s (ACC : Acc lt (size_shadow s)) {struct ACC} : trace :=
     match s as s' return s = s' -> _ with
-    | Init => fun _ => Some (vl_exp σ)
-    | Read s x =>
-      fun _ =>
-      let folds s :=
-        match s with
-        | vl_exp σ => lift (Some <*> unroll) (read_env σ x)
-        | vl_sh (SuccS _) | vl_sh (PredS _) => None
-        | vl_sh s => Some (vl_sh (Read s x))
-        | vl_clos _ _ _ | vl_nat _ => None
-        end
-      in lift folds (link_shdw s (Acc_inv ACC _))
-    | Call s v =>
-      fun _ =>
-      let folds s :=
-        let foldv v :=
-          match s with
-          | vl_clos x k σ =>
-            lift (link n (nv_bval x (wvl_v v) σ)) k
-          | vl_sh (SuccS _) | vl_sh (PredS _) => None
-          | vl_sh s => Some (vl_sh (Call s v))
-          | vl_exp _ | vl_nat _ => None
-          end
-        in lift foldv (link_vl v (Acc_inv ACC _))
-      in lift folds (link_shdw s (Acc_inv ACC _))
-    | SuccS s =>
-      fun _ =>
-      let folds s :=
-        match s with
-        | vl_nat n => Some (vl_nat (S n))
-        | vl_sh (PredS s) => Some (vl_sh s)
-        | vl_sh s => Some (vl_sh (SuccS s))
-        | vl_exp _ | vl_clos _ _ _ => None
-        end
-      in lift folds (link_shdw s (Acc_inv ACC _))
-    | PredS s =>
-      fun _ =>
-      let folds s :=
-        match s with
-        | vl_nat (S n) => Some (vl_nat n)
-        | vl_sh (SuccS s) => Some (vl_sh s)
-        | vl_sh s => Some (vl_sh (PredS s))
-        | vl_nat O | vl_exp _ | vl_clos _ _ _ => None
-        end
-      in lift folds (link_shdw s (Acc_inv ACC _))
-    | CaseS s vO vS =>
-      fun _ =>
-      let folds s :=
-        let vO :=
-          match vO as vO' return vO = vO' -> _ with
-          | None => fun _ => None
-          | Some vO => fun _ => link_vl vO (Acc_inv ACC _)
-          end eq_refl in
-        let vS :=
-          match vS as vS' return vS = vS' -> _ with
-          | None => fun _ => None
-          | Some vS => fun _ => link_vl vS (Acc_inv ACC _)
-          end eq_refl in
-        match s with
-        | vl_nat O => vO
-        | vl_nat (S _) | vl_sh (SuccS _) => vS
-        | vl_sh s => Some (vl_sh (CaseS s vO vS))
-        | vl_exp _ | vl_clos _ _ _ => None
-        end
-      in lift folds (link_shdw s (Acc_inv ACC _))
+    | Init => fun _ => Wal (wvl_v (vl_exp σ))
+    | Read s x => fun _ =>
+      read_trace x (link_shdw s (Acc_inv ACC _))
+    | Call s w => fun _ =>
+      let fn := link_shdw s (Acc_inv ACC _) in
+      let arg := link_wvl w (Acc_inv ACC _) in
+      call_trace (link n) fn arg
+    | Dstr s d => fun _ =>
+      dstr_trace d (link_shdw s (Acc_inv ACC _))
     end eq_refl
-  for link_vl
-  in fun v => go v (lt_wf (size_value v))
+  for link_wvl
+  in fun w => go w (lt_wf (size_walue w))
   end).
   Unshelve.
   all: try abstract t.
   all: abstract t.
 Defined.
 
+Definition eval (link : env -> walue -> trace) :=
+  fix eval (e : tm) : trace :=
+  match e with
+  | Var x => Guard (nv_sh Init) (Wal (wvl_v (vl_sh (Read Init x))))
+  | Fn x M => Guard (nv_sh Init) (Wal (wvl_v (vl_clos x (eval M) (nv_sh Init))))
+  | App M N => call_trace link (eval M) (eval N)
+  | Link M N =>
+    let client := eval N in
+    let check_module m :=
+      match unroll m with
+      | Some (vl_sh s) => link_trace (link (nv_sh s)) Wal client
+      | Some (vl_exp σ) => link_trace (link σ) Wal client
+      | _ => Bot
+      end
+    in bind check_module (eval M)
+  | Mt => Guard (nv_sh Init) (Wal (wvl_v (vl_exp nv_mt)))
+  | Bind x M N =>
+    let bd := eval M in
+    let exp := eval N in
+    let check_bd w :=
+      match unroll w with
+      | Some v =>
+        let w := wvl_recv (close_value 0 xH v) in
+        let check_exp σ :=
+          match unroll σ with
+          | Some (vl_sh s) => Wal (wvl_v (vl_exp (nv_bd x w (nv_sh s))))
+          | Some (vl_exp σ) => Wal (wvl_v (vl_exp (nv_bd x w σ)))
+          | _ => Bot
+          end
+        in link_trace (link (nv_bd x w (nv_sh Init))) check_exp exp
+      | None => Bot
+      end
+    in link_trace (link (nv_bd x (wvl_floc xH) (nv_sh Init))) check_bd bd
+  | Cstr c =>
+    cstr_trace
+      {|
+        cs_type := c.(cs_type);
+        cs_args := map_vec eval c.(cs_args)
+      |}
+  | Case E B =>
+    let matched := eval E in
+    let branches :=
+      let for_each b :=
+        {|
+          br_cstr := b.(br_cstr);
+          br_vars := b.(br_vars);
+          br_body := eval b.(br_body);
+        |} in
+      List.map for_each B in
+    let check_match m :=
+      match unroll m with
+      | Some (vl_sh s) =>
+        let for_each b :=
+          let body := link_trace (link (dstr_shadow s b)) Wal b.(br_body)
+          in (b.(br_cstr), body)
+        in Match s (List.map for_each branches)
+      | Some (vl_cstr c) =>
+        let fold_each acc b :=
+          match acc with
+          | None =>
+            match dstr_cstr c b with
+            | None => None
+            | Some σ => Some (link_trace (link σ) Wal b.(br_body))
+            end
+          | Some t => Some t
+          end
+        in match List.fold_left fold_each branches None with
+        | None => Bot
+        | Some t => t
+        end
+      | _ => Bot
+      end
+    in bind check_match matched
+  end.
+
 Definition interp n := eval (link n).
 
-Local Coercion wvl_v : vl >-> wvl.
+Fixpoint get_wal t :=
+  match t with
+  | Bot => []
+  | Wal w => [w]
+  | Match _ b =>
+    let fold acc (b : cstr_type * trace) :=
+      let (c, t) := b in get_wal t ++ acc
+    in List.fold_left fold b nil
+  | Guard _ t => get_wal t
+  end%list.
+
 Local Coercion vl_exp : nv >-> vl.
-Definition one_tm := Succ Zero.
-Definition two_tm := Succ (Succ Zero).
-Definition three_tm := Succ (Succ (Succ Zero)).
+Definition zero_tm c :=
+  Cstr {|
+    cs_type := {| cs_name := c; cs_arity := 0 |};
+    cs_args := []%vec;
+  |}.
+Definition succ_tm t :=
+  Cstr {|
+    cs_type := {| cs_name := Succ; cs_arity := 1 |};
+    cs_args := [t]%vec;
+  |}.
+Definition one_tm := succ_tm (zero_tm Zero).
+Definition two_tm := succ_tm one_tm.
+Definition three_tm := succ_tm two_tm.
 (* Fixpoint add m n := match m with 0 => n | S m => S (add m n) end *)
+Definition zero_branch (t : tm) :=
+  {|
+    br_cstr := {| cs_name := Zero; cs_arity := _ |};
+    br_vars := []%vec;
+    br_body := t
+  |}.
+Definition succ_branch x (t : tm) :=
+  {|
+    br_cstr := {| cs_name := Succ; cs_arity := _ |};
+    br_vars := [x]%vec;
+    br_body := t
+  |}.
 Definition add_tm :=
 Link (Bind "+"
   (Fn "m"
     (Fn "n"
       (Case (Var "m")
-        (Var "n")
-        "m"
-        (Succ (App (App (Var "+") (Var "m")) (Var "n"))))))
+        [zero_branch (Var "n");
+        succ_branch "m" (succ_tm (App (App (Var "+") (Var "m")) (Var "n")))]
+      )))
   Mt) (Var "+")
 .
 
-Definition three_plus_three := App (App add_tm three_tm) three_tm.
+Compute get_wal (interp 10 (App add_tm (zero_tm Zero))).
 
-Definition x_plus_three := App (App add_tm three_tm) (Var "x").
+Compute get_wal
+  (interp 10 (App (App add_tm (zero_tm Zero)) (zero_tm Zero))).
 
-Definition double_x := App (App add_tm (Var "x")) (Var "x").
+Module MutExample.
+(* even? n = 1 if n is even 0 if n is odd *)
+Definition top_module :=
+Bind "Top"
+  (Bind "Even"
+    (Bind "even?"
+      (Fn "x"
+        (Case (Var "x")
+          [zero_branch (zero_tm One);
+          succ_branch "n" (App (Link (Var "Top") (Link (Var "Odd") (Var "odd?"))) (Var "n"))]
+        ))
+      Mt)
+    (Bind "Odd"
+      (Bind "odd?"
+        (Fn "y"
+          (Case (Var "y")
+            [zero_branch (zero_tm Zero);
+            succ_branch "n" (App (Link (Var "Top") (Link (Var "Even") (Var "even?"))) (Var "n"))]
+          ))
+        Mt)
+      Mt))
+  Mt.
 
-Compute interp 5 three_plus_three.
-Compute interp 6 x_plus_three.
-Compute interp 6 double_x.
-Compute interp 100
-  (App
-    (App add_tm
-      (App
-        (App add_tm one_tm)
-        two_tm))
-    (Var "x")).
+Definition test_even :=
+  Link top_module
+    (Link (Var "Top") (Link (Var "Even") (Var "even?"))).
+Definition test_odd :=
+  Link top_module
+    (Link (Var "Top") (Link (Var "Odd") (Var "odd?"))).
 
-Definition sum_tm :=
-Link (Bind "Σ"
-  (Fn "f"
-    (Fn "n"
-      (Case (Var "n")
-        (App (Var "f") Zero)
-        "n"
-        (App
-          (App (Var "+") (App (Var "f") (Succ (Var "n"))))
-          (App
-            (App (Var "Σ") (Var "f"))
-            (Var "n"))))))
-  Mt) (Var "Σ").
+Compute get_wal (interp 10 top_module).
 
-Definition unknown_function :=
-  App (App sum_tm (Var "f")) three_tm.
+Compute get_wal (interp 10 test_even).
 
-Compute interp 5 unknown_function.
+Definition test_num := three_tm.
 
-Definition unknown_function_and_number :=
-  App (App sum_tm (Var "f")) (Var "n").
-
-Compute interp 5 unknown_function_and_number.
-
-Definition unknown_function_and_number_sem :=
-  Eval vm_compute in
-  interp 5 (App (App sum_tm (Var "f")) (Var "n")).
-
-Print unknown_function_and_number_sem.
-
-Definition sem_link n (σ : option nv) (v : option vl) :=
-  match σ with
-  | None => None
-  | Some σ => lift (link n σ) v
-  end.
-
-Compute sem_link 5 (Some (nv_bval "n" (wvl_v (vl_nat 3)) (nv_sh Init)))
-  unknown_function_and_number_sem.
-
-Compute interp 100
-  (Link (Bind "+" add_tm (Bind "n" three_tm (Bind "f" (Fn "x" (Var "x")) Mt)))
-        unknown_function_and_number).
-
-Compute interp 10
-(App
-  (App add_tm
-    (App (App add_tm (Var "x")) (Succ Zero)))
-    (Succ (Succ Zero))).
+Compute get_wal (interp 10 (App test_even test_num)).
+Compute get_wal (interp 10 (App test_odd test_num)).
+Compute get_wal (interp 10 (App test_odd (Var "n"))).
+End MutExample.
 
